benchmarks/tests.v
@@ -18,6 +18,7 @@ Definition demo2 := List.map negb [true; false; true].
 Definition demo3 := andb. 
   
 CertiCoq Compile -ext "_cps" demo1.
+CertiCoq Show IR -ext "_cps" demo1.
 CertiCoq Compile -anf demo1.
 
 CertiCoq Compile -ext "_cps" demo2.
@@ -45,7 +46,7 @@ Definition vs_hard :=
   | _ => false
   end.
 
-CertiCoq Compile -ext "_cps" -time vs_easy.
+(* CertiCoq Compile -ext "_cps" -time vs_easy. *)
 CertiCoq Compile -anf  vs_easy.
 
 (* Zoe: Compiling with the CPS pipeline takes much longer for vs_easy.
@@ -72,7 +73,7 @@ Debug: Time elapsed in L6 ANF:  0.020384
 Debug: Time elapsed in L6 Pipeline:  0.148308
 Debug: Time elapsed in L7:  2.394216 *)
 
-CertiCoq Compile -ext "_cps" vs_hard.
+(* CertiCoq Compile -ext "_cps" vs_hard. *)
 CertiCoq Compile -anf vs_hard.
 
 Definition binom := Binom.main.
@@ -82,5 +83,5 @@ CertiCoq Compile -anf binom.  (* returns nat *)
 
 Definition color := Color.main.
 
-CertiCoq Compile -ext "_cps" color.
+(* CertiCoq Compile -ext "_cps" color. *)
 CertiCoq Compile -anf color.
